Lean4Lean/Theory/Typing/ParallelReduction.lean
@@ -9,12 +9,11 @@ namespace Lean4Lean
 
 open VExpr
 
-def Extra := List VExpr → VExpr → VExpr → VExpr → VExpr → Prop
-
 section
 set_option hygiene false
+variable (TY : Typing)
 local notation:65 Γ " ⊢ " e1 " ≫ " e2:30 => ParRed Γ e1 e2
-variable (extra : Extra)
+local notation:65 Γ " ⊢ " e1 " ⋙ " e2:30 => CParRed Γ e1 e2
 
 inductive ParRed : List VExpr → VExpr → VExpr → Prop where
   | bvar : Γ ⊢ .bvar i ≫ .bvar i
@@ -24,68 +23,197 @@ inductive ParRed : List VExpr → VExpr → VExpr → Prop where
   | lam : Γ ⊢ A ≫ A' → A::Γ ⊢ body ≫ body' → Γ ⊢ .lam A body ≫ .lam A' body'
   | forallE : Γ ⊢ A ≫ A' → A::Γ ⊢ B ≫ B' → Γ ⊢ .forallE A B ≫ .forallE A' B'
   | beta : A::Γ ⊢ e₁ ≫ e₁' → Γ ⊢ e₂ ≫ e₂' → Γ ⊢ .app (.lam A e₁) e₂ ≫ e₁'.inst e₂'
-  | extra : (∀ a a', extra Γ e e' a a' → Γ ⊢ a ≫ a') → Γ ⊢ e ≫ e'
+  | extra : TY.Pat p r → p.Matches e m1 m2 → r.2.OK (TY.IsDefEq Γ) m1 m2 →
+    (∀ a, Γ ⊢ m2 a ≫ m2' a) → Γ ⊢ e ≫ r.1.apply m1 m2'
+
+def IsNeutral (Γ : List VExpr) (e : VExpr) : Prop :=
+  (∀ A e₁ e₂, e ≠ .app (.lam A e₁) e₂) ∧
+  (∀ p r m1 m2, TY.Pat p r → p.Matches e m1 m2 → ¬r.2.OK (TY.IsDefEq Γ) m1 m2)
+
+inductive CParRed : List VExpr → VExpr → VExpr → Prop where
+  | bvar : Γ ⊢ .bvar i ⋙ .bvar i
+  | sort : Γ ⊢ .sort u ⋙ .sort u
+  | const : IsNeutral TY Γ (.const c ls) → Γ ⊢ .const c ls ⋙ .const c ls
+  | app : IsNeutral TY Γ (.app f a) → Γ ⊢ f ⋙ f' → Γ ⊢ a ⋙ a' → Γ ⊢ .app f a ⋙ .app f' a'
+  | lam : Γ ⊢ A ⋙ A' → A::Γ ⊢ body ⋙ body' → Γ ⊢ .lam A body ⋙ .lam A' body'
+  | forallE : Γ ⊢ A ⋙ A' → A::Γ ⊢ B ⋙ B' → Γ ⊢ .forallE A B ⋙ .forallE A' B'
+  | beta : A::Γ ⊢ e₁ ⋙ e₁' → Γ ⊢ e₂ ⋙ e₂' → Γ ⊢ .app (.lam A e₁) e₂ ⋙ e₁'.inst e₂'
+  | extra : TY.Pat p r → p.Matches e m1 m2 → r.2.OK (TY.IsDefEq Γ) m1 m2 →
+    (∀ a, Γ ⊢ m2 a ⋙ m2' a) → Γ ⊢ e ⋙ r.1.apply m1 m2'
 
 end
 
-theorem ParRed.rfl : ∀ {e}, ParRed E Γ e e
+variable {TY : Typing}
+
+protected theorem ParRed.rfl : ∀ {e}, ParRed TY Γ e e
   | .bvar .. => .bvar
   | .sort .. => .sort
   | .const .. => .const
-  | .app .. => .app rfl rfl
-  | .lam .. => .lam rfl rfl
-  | .forallE .. => .forallE rfl rfl
+  | .app .. => .app ParRed.rfl ParRed.rfl
+  | .lam .. => .lam ParRed.rfl ParRed.rfl
+  | .forallE .. => .forallE ParRed.rfl ParRed.rfl
 
-def Extra.IsWeakN (E : Extra) :=
-  ∀ {{Γ e e' a a' Γ' n k}},
-    Ctx.LiftN n k Γ Γ' → E Γ' (liftN n e k) (liftN n e' k) a a' →
-    ∃ b b', E Γ e e' b b' ∧ a = liftN n b k ∧ a' = liftN n b' k
-
-variable (HE : Extra.IsWeakN E) in
-theorem ParRed.weakN (W : Ctx.LiftN n k Γ Γ') (H : ParRed E Γ e1 e2) :
-    ParRed E Γ' (e1.liftN n k) (e2.liftN n k) := by
+theorem ParRed.weakN (W : Ctx.LiftN n k Γ Γ') (H : ParRed TY Γ e1 e2) :
+    ParRed TY Γ' (e1.liftN n k) (e2.liftN n k) := by
   induction H generalizing k Γ' with
-  | bvar | sort | const => exact rfl
+  | bvar | sort | const => exact .rfl
   | app _ _ ih1 ih2 => exact .app (ih1 W) (ih2 W)
   | lam _ _ ih1 ih2 => exact .lam (ih1 W) (ih2 W.succ)
   | forallE _ _ ih1 ih2 => exact .forallE (ih1 W) (ih2 W.succ)
   | beta _ _ ih1 ih2 =>
     simp [liftN, liftN_inst_hi]
     exact .beta (ih1 W.succ) (ih2 W)
-  | extra _ ih =>
-    refine .extra fun a a' h => ?_
-    obtain ⟨_, _, h', rfl, rfl⟩ := HE W h
-    exact ih _ _ h' W
+  | extra h1 h2 h3 _ ih =>
+    rw [Pattern.RHS.liftN_apply]
+    refine .extra h1 (Pattern.matches_liftN.2 ⟨_, h2, funext_iff.1 rfl⟩)
+      (h3.weakN W) (fun a => ih _ W)
 
-def Extra.IsInstN (E : Extra) :=
-  E.IsWeakN ∧
-  ∀ {{Γ₀ Γ₁ Γ A₀ k e1 e2 a1 a2 x1 x2}},
-    Ctx.InstN Γ₀ a1 A₀ k Γ₁ Γ → E Γ (inst e1 a1 k) (inst e2 a2 k) x1 x2 →
-    ∃ b1 b2, E Γ₁ e1 e2 b1 b2 ∧ x1 = inst b1 a1 k ∧ x2 = inst b2 a2 k
-
-variable (HE : Extra.IsInstN E) (H0 : ParRed E Γ₀ a1 a2) in
+variable (H₀ : ParRed TY Γ₀ a1 a2) (H₀' : TY.HasType Γ₀ a1 A₀) in
 theorem ParRed.instN (W : Ctx.InstN Γ₀ a1 A₀ k Γ₁ Γ)
-    (H : ParRed E Γ₁ e1 e2) : ParRed E Γ (e1.inst a1 k) (e2.inst a2 k) := by
+    (H : ParRed TY Γ₁ e1 e2) : ParRed TY Γ (e1.inst a1 k) (e2.inst a2 k) := by
   induction H generalizing Γ k with
   | @bvar _ i =>
     dsimp [inst]
     induction W generalizing i with
     | zero =>
       cases i with simp [inst_lift]
-      | zero => exact H0
-      | succ h => exact rfl
+      | zero => exact H₀
+      | succ h => exact .rfl
     | succ _ ih =>
       cases i with simp
-      | zero => exact rfl
-      | succ h => exact ih.weakN HE.1 .one
-  | sort | const => exact rfl
+      | zero => exact .rfl
+      | succ h => exact ih.weakN .one
+  | sort | const => exact .rfl
   | app _ _ ih1 ih2 => exact .app (ih1 W) (ih2 W)
   | lam _ _ ih1 ih2 => exact .lam (ih1 W) (ih2 W.succ)
   | forallE _ _ ih1 ih2 => exact .forallE (ih1 W) (ih2 W.succ)
   | beta _ _ ih1 ih2 =>
     simp [inst, inst0_inst_hi]
     exact .beta (ih1 W.succ) (ih2 W)
-  | extra _ ih =>
-    refine .extra fun a a' h => ?_
-    obtain ⟨_, _, h', rfl, rfl⟩ := HE.2 W h
-    exact ih _ _ h' W
+  | extra h1 h2 h3 _ ih =>
+    rw [Pattern.RHS.instN_apply]
+    exact .extra h1 (Pattern.matches_instN h2) (h3.instN W H₀') (fun a => ih _ W)
+
+theorem ParRed.defeq (H : ParRed TY Γ e e') (he : TY.HasType Γ e A) : TY.IsDefEq Γ e e' := by
+  induction H generalizing A with
+  | bvar | sort | const => exact TY.refl he
+  | app _ _ ih1 ih2 =>
+    have ⟨_, _, h1, h2⟩ := TY.app_inv he
+    exact TY.appDF h1 (ih1 h1) h2 (ih2 h2)
+  | lam _ _ ih1 ih2 =>
+    have ⟨_, _, h1, h2⟩ := TY.lam_inv he
+    exact TY.lamDF h1 (ih1 h1) (ih2 h2)
+  | forallE _ _ ih1 ih2 =>
+    have ⟨_, _, h1, h2⟩ := TY.forallE_inv he
+    exact TY.forallEDF h1 (ih1 h1) h2 (ih2 h2)
+  | beta _ _ ih1 ih2 =>
+    have ⟨_, _, hf, ha⟩ := TY.app_inv he
+    have ⟨_, _, hA, hb⟩ := TY.lam_inv hf
+    have hf' := TY.lam hA hb
+    replace ha := TY.defeq_r (TY.forallE_defInv (TY.uniq hf hf')).1 ha
+    exact TY.trans (TY.appDF hf' (TY.lamDF hA (TY.refl hA) (ih1 hb)) ha (ih2 ha))
+      (TY.beta (TY.defeq_l (ih1 hb) hb) (TY.defeq_l (ih2 ha) ha))
+  | @extra p r e m1 m2 Γ m2' h1 h2 h3 _ ih =>
+    exact TY.trans (TY.pat_wf h1 h2 he h3) <|
+     .apply_pat ih (TY.defeq_l (TY.pat_wf h1 h2 he h3) he)
+
+theorem ParRed.hasType (H : ParRed TY Γ e e') (he : TY.HasType Γ e A) : TY.HasType Γ e' A :=
+  TY.defeq_l (H.defeq he) he
+
+theorem ParRed.defeqDFC (W : IsDefEqCtx TY.IsDefEq Γ₀ Γ₁ Γ₂)
+    (h : TY.HasType Γ₁ e1 A) (H : ParRed TY Γ₁ e1 e2) : ParRed TY Γ₂ e1 e2 := by
+  induction H generalizing Γ₂ A with
+  | bvar => exact .bvar
+  | sort => exact .sort
+  | const => exact .const
+  | app _ _ ih1 ih2 =>
+    have ⟨_, _, hf, ha⟩ := TY.app_inv h
+    exact .app (ih1 W hf) (ih2 W ha)
+  | lam _ _ ih1 ih2 =>
+    have ⟨_, _, hA, he⟩ := TY.lam_inv h
+    exact .lam (ih1 W hA) (ih2 (W.succ (TY.refl hA)) he)
+  | forallE _ _ ih1 ih2 =>
+    have ⟨_, _, hA, hB⟩ := TY.forallE_inv h
+    exact .forallE (ih1 W hA) (ih2 (W.succ (TY.refl hA)) hB)
+  | beta _ _ ih1 ih2 =>
+    have ⟨_, _, hf, ha⟩ := TY.app_inv h
+    have ⟨_, _, hA, hb⟩ := TY.lam_inv hf
+    exact .beta (ih1 (W.succ (TY.refl hA)) hb) (ih2 W ha)
+  | @extra p r e m1 m2 Γ m2' h1 h2 h3 _ ih =>
+    exact .extra h1 h2 (h3.map fun a b h => TY.isDefEq_DFC W h) fun a =>
+      let ⟨_, h⟩ := h2.hasType h a; ih a W h
+
+
+theorem ParRed.apply_pat {p : Pattern} (r : p.RHS) {m1 m2 m3}
+    (H : ∀ a, ParRed TY Γ (m2 a) (m3 a)) : ParRed TY Γ (r.apply m1 m2) (r.apply m1 m3) := by
+  match r with
+  | .fixed .. => exact .rfl
+  | .app f a => exact .app (apply_pat f H) (apply_pat a H)
+  | .var f => exact H _
+
+theorem CParRed.toParRed (H : CParRed TY Γ e e') : ParRed TY Γ e e' := by
+  induction H with
+  | bvar => exact .bvar
+  | sort => exact .sort
+  | const => exact .const
+  | app _ _ _ ih1 ih2 => exact .app ih1 ih2
+  | lam _ _ ih1 ih2 => exact .lam ih1 ih2
+  | forallE _ _ ih1 ih2 => exact .forallE ih1 ih2
+  | beta _ _ ih1 ih2 => exact .beta ih1 ih2
+  | extra h1 h2 h3 _ ih3 => exact .extra h1 h2 h3 ih3
+
+theorem CParRed.exists (H : TY.HasType Γ e A) : ∃ e', CParRed TY Γ e e' := by
+  induction e using VExpr.brecOn generalizing Γ A with | _ e e_ih => ?_
+  have neut e
+      (H' : TY.HasType Γ e A)
+      (e_ih : VExpr.below (motive := fun {e} =>
+        ∀ {Γ A}, TY.HasType Γ e A → ∃ e', CParRed TY Γ e e') e)
+      (hn : IsNeutral TY Γ e → ∃ e', CParRed TY Γ e e') : ∃ e', CParRed TY Γ e e' := by
+    by_cases h : ∃ A e₁ e₂, e = .app (.lam A e₁) e₂
+    · obtain ⟨A, e, a, rfl⟩ := h
+      have ⟨_, _, hf, ha⟩ := TY.app_inv H'
+      have ⟨_, _, _, he⟩ := TY.lam_inv hf
+      have ⟨_, he⟩ := e_ih.1.2.2.1.1 he
+      have ⟨_, ha⟩ := e_ih.2.1.1 ha
+      exact ⟨_, .beta he ha⟩
+    by_cases h' : ∃ p r m1 m2, TY.Pat p r ∧ p.Matches e m1 m2 ∧ r.2.OK (TY.IsDefEq Γ) m1 m2
+    · let ⟨p, r, m1, m2, h1, hp2, hp3⟩ := h'
+      suffices ∃ m3 : p.Path.2 → VExpr, ∀ a, CParRed TY Γ (m2 a) (m3 a) from
+        let ⟨_, h3⟩ := this; ⟨_, .extra h1 hp2 hp3 h3⟩
+      clear H hn h h' r h1 hp3
+      induction p generalizing e A with
+      | const => exact ⟨nofun, nofun⟩
+      | app f a ih1 ih2 =>
+        let .app hm1 hm2 := hp2
+        have ⟨_, _, H1, H2⟩ := TY.app_inv H'
+        have ⟨m2l, hl⟩ := ih1 _ H1 e_ih.1.2 _ _ hm1
+        have ⟨m2r, hr⟩ := ih2 _ H2 e_ih.2.1.2 _ _ hm2
+        exact ⟨Sum.elim m2l m2r, Sum.rec hl hr⟩
+      | var _ ih =>
+        let .var hm1 := hp2
+        have ⟨_, _, H1, H2⟩ := TY.app_inv H'
+        have ⟨m2l, hl⟩ := ih _ H1 e_ih.1.2 _ _ hm1
+        have ⟨e', hs⟩ := e_ih.2.1.1 H2
+        exact ⟨Option.rec e' m2l, Option.rec hs hl⟩
+    · exact hn ⟨
+        fun _ _ _ hn => h ⟨_, _, _, hn⟩,
+        fun _ _ _ _ h1 h2 h3 => h' ⟨_, _, _, _, h1, h2, h3⟩⟩
+  cases e with
+  | bvar i => exact ⟨_, .bvar⟩
+  | sort => exact ⟨_, .sort⟩
+  | const n ls => exact neut _ H e_ih fun hn => ⟨_, .const hn⟩
+  | app ih1 ih2 =>
+    have ⟨_, _, hf, ha⟩ := TY.app_inv H
+    have ⟨_, h1⟩ := e_ih.1.1 hf
+    have ⟨_, h2⟩ := e_ih.2.1.1 ha
+    exact neut _ H e_ih fun hn => ⟨_, .app hn h1 h2⟩
+  | lam ih1 ih2 =>
+    have ⟨_, _, hA, he⟩ := TY.lam_inv H
+    have ⟨_, h1⟩ := e_ih.1.1 hA
+    have ⟨_, h2⟩ := e_ih.2.1.1 he
+    exact ⟨_, .lam h1 h2⟩
+  | forallE ih1 ih2 =>
+    have ⟨_, _, hA, hB⟩ := TY.forallE_inv H
+    have ⟨_, h1⟩ := e_ih.1.1 hA
+    have ⟨_, h2⟩ := e_ih.2.1.1 hB
+    exact ⟨_, .forallE h1 h2⟩
